rename

Arithmetization/ISigmaOne/Metamath/Formula/Typed.lean
@@ -31,19 +31,19 @@ section typed_formula
 
 variable (L)
 
-structure Language.TSemiformula (n : V) where
+structure Language.Semiformula (n : V) where
   val : V
   prop : L.IsSemiformula n val
 
-attribute [simp] Language.TSemiformula.prop
+attribute [simp] Language.Semiformula.prop
 
-abbrev Language.TFormula := L.TSemiformula 0
+abbrev Language.TFormula := L.Semiformula 0
 
 variable {L}
 
-@[simp] lemma Language.TSemiformula.isUFormula (p : L.TSemiformula n) : L.IsUFormula p.val := p.prop.isUFormula
+@[simp] lemma Language.Semiformula.isUFormula (p : L.Semiformula n) : L.IsUFormula p.val := p.prop.isUFormula
 
-scoped instance : LogicalConnective (L.TSemiformula n) where
+scoped instance : LogicalConnective (L.Semiformula n) where
   top := ⟨^⊤, by simp⟩
   bot := ⟨^⊥, by simp⟩
   wedge (p q) := ⟨p.val ^⋏ q.val, by simp⟩
@@ -51,153 +51,153 @@ scoped instance : LogicalConnective (L.TSemiformula n) where
   tilde (p) := ⟨L.neg p.val, by simp⟩
   arrow (p q) := ⟨L.imp p.val q.val, by simp⟩
 
-def Language.TSemiformula.cast (p : L.TSemiformula n) (eq : n = n' := by simp) : L.TSemiformula n' := eq ▸ p
+def Language.Semiformula.cast (p : L.Semiformula n) (eq : n = n' := by simp) : L.Semiformula n' := eq ▸ p
 
-@[simp] lemma Language.TSemiformula.val_cast (p : L.TSemiformula n) (eq : n = n') :
-    (p.cast eq).val = p.val := by rcases eq; simp [Language.TSemiformula.cast]
+@[simp] lemma Language.Semiformula.val_cast (p : L.Semiformula n) (eq : n = n') :
+    (p.cast eq).val = p.val := by rcases eq; simp [Language.Semiformula.cast]
 
-def Language.TSemiformula.all (p : L.TSemiformula (n + 1)) : L.TSemiformula n := ⟨^∀ p.val, by simp⟩
+def Language.Semiformula.all (p : L.Semiformula (n + 1)) : L.Semiformula n := ⟨^∀ p.val, by simp⟩
 
-def Language.TSemiformula.ex (p : L.TSemiformula (n + 1)) : L.TSemiformula n := ⟨^∃ p.val, by simp⟩
+def Language.Semiformula.ex (p : L.Semiformula (n + 1)) : L.Semiformula n := ⟨^∃ p.val, by simp⟩
 
-namespace Language.TSemiformula
+namespace Language.Semiformula
 
-@[simp] lemma val_verum : (⊤ : L.TSemiformula n).val = ^⊤ := rfl
+@[simp] lemma val_verum : (⊤ : L.Semiformula n).val = ^⊤ := rfl
 
-@[simp] lemma val_falsum : (⊥ : L.TSemiformula n).val = ^⊥ := rfl
+@[simp] lemma val_falsum : (⊥ : L.Semiformula n).val = ^⊥ := rfl
 
-@[simp] lemma val_and (p q : L.TSemiformula n) :
+@[simp] lemma val_and (p q : L.Semiformula n) :
     (p ⋏ q).val = p.val ^⋏ q.val := rfl
 
-@[simp] lemma val_or (p q : L.TSemiformula n) :
+@[simp] lemma val_or (p q : L.Semiformula n) :
     (p ⋎ q).val = p.val ^⋎ q.val := rfl
 
-@[simp] lemma val_neg (p : L.TSemiformula n) :
+@[simp] lemma val_neg (p : L.Semiformula n) :
     (~p).val = L.neg p.val := rfl
 
-@[simp] lemma val_imp (p q : L.TSemiformula n) :
+@[simp] lemma val_imp (p q : L.Semiformula n) :
     (p ⟶ q).val = L.imp p.val q.val := rfl
 
-@[simp] lemma val_all (p : L.TSemiformula (n + 1)) :
+@[simp] lemma val_all (p : L.Semiformula (n + 1)) :
     p.all.val = ^∀ p.val := rfl
 
-@[simp] lemma val_ex (p : L.TSemiformula (n + 1)) :
+@[simp] lemma val_ex (p : L.Semiformula (n + 1)) :
     p.ex.val = ^∃ p.val := rfl
 
-lemma val_inj {p q : L.TSemiformula n} :
+lemma val_inj {p q : L.Semiformula n} :
     p.val = q.val ↔ p = q := by rcases p; rcases q; simp
 
-@[ext] lemma ext {p q : L.TSemiformula n} (h : p.val = q.val) : p = q := val_inj.mp h
+@[ext] lemma ext {p q : L.Semiformula n} (h : p.val = q.val) : p = q := val_inj.mp h
 
-lemma ext_iff {p q : L.TSemiformula n} : p = q ↔ p.val = q.val := by rcases p; rcases q; simp
+lemma ext_iff {p q : L.Semiformula n} : p = q ↔ p.val = q.val := by rcases p; rcases q; simp
 
-@[simp] lemma and_inj {p₁ p₂ q₁ q₂ : L.TSemiformula n} :
+@[simp] lemma and_inj {p₁ p₂ q₁ q₂ : L.Semiformula n} :
     p₁ ⋏ p₂ = q₁ ⋏ q₂ ↔ p₁ = q₁ ∧ p₂ = q₂ := by simp [ext_iff]
 
-@[simp] lemma or_inj {p₁ p₂ q₁ q₂ : L.TSemiformula n} :
+@[simp] lemma or_inj {p₁ p₂ q₁ q₂ : L.Semiformula n} :
     p₁ ⋎ p₂ = q₁ ⋎ q₂ ↔ p₁ = q₁ ∧ p₂ = q₂ := by simp [ext_iff]
 
-@[simp] lemma all_inj {p q : L.TSemiformula (n + 1)} :
+@[simp] lemma all_inj {p q : L.Semiformula (n + 1)} :
     p.all = q.all ↔ p = q := by simp [ext_iff]
 
-@[simp] lemma ex_inj {p q : L.TSemiformula (n + 1)} :
+@[simp] lemma ex_inj {p q : L.Semiformula (n + 1)} :
     p.ex = q.ex ↔ p = q := by simp [ext_iff]
 
-@[simp] lemma neg_verum : ~(⊤ : L.TSemiformula n) = ⊥ := by ext; simp
-@[simp] lemma neg_falsum : ~(⊥ : L.TSemiformula n) = ⊤ := by ext; simp
-@[simp] lemma neg_and (p q : L.TSemiformula n) : ~(p ⋏ q) = ~p ⋎ ~q := by ext; simp
-@[simp] lemma neg_or (p q : L.TSemiformula n) : ~(p ⋎ q) = ~p ⋏ ~q := by ext; simp
-@[simp] lemma neg_all (p : L.TSemiformula (n + 1)) : ~p.all = (~p).ex := by ext; simp
-@[simp] lemma neg_ex (p : L.TSemiformula (n + 1)) : ~p.ex = (~p).all := by ext; simp
+@[simp] lemma neg_verum : ~(⊤ : L.Semiformula n) = ⊥ := by ext; simp
+@[simp] lemma neg_falsum : ~(⊥ : L.Semiformula n) = ⊤ := by ext; simp
+@[simp] lemma neg_and (p q : L.Semiformula n) : ~(p ⋏ q) = ~p ⋎ ~q := by ext; simp
+@[simp] lemma neg_or (p q : L.Semiformula n) : ~(p ⋎ q) = ~p ⋏ ~q := by ext; simp
+@[simp] lemma neg_all (p : L.Semiformula (n + 1)) : ~p.all = (~p).ex := by ext; simp
+@[simp] lemma neg_ex (p : L.Semiformula (n + 1)) : ~p.ex = (~p).all := by ext; simp
 
-lemma imp_def (p q : L.TSemiformula n) : p ⟶ q = ~p ⋎ q := by ext; simp [imp]
+lemma imp_def (p q : L.Semiformula n) : p ⟶ q = ~p ⋎ q := by ext; simp [imp]
 
-@[simp] lemma neg_neg (p : L.TSemiformula n) : ~~p = p := by
+@[simp] lemma neg_neg (p : L.Semiformula n) : ~~p = p := by
   ext; simp [shift, Language.IsUFormula.neg_neg]
 
-def shift (p : L.TSemiformula n) : L.TSemiformula n := ⟨L.shift p.val, p.prop.shift⟩
+def shift (p : L.Semiformula n) : L.Semiformula n := ⟨L.shift p.val, p.prop.shift⟩
 
-def substs (p : L.TSemiformula n) (w : L.TSemitermVec n m) : L.TSemiformula m :=
+def substs (p : L.Semiformula n) (w : L.TSemitermVec n m) : L.Semiformula m :=
   ⟨L.substs w.val p.val, p.prop.substs w.prop⟩
 
-@[simp] lemma val_shift (p : L.TSemiformula n) : p.shift.val = L.shift p.val := rfl
-@[simp] lemma val_substs (p : L.TSemiformula n) (w : L.TSemitermVec n m) : (p.substs w).val = L.substs w.val p.val := rfl
+@[simp] lemma val_shift (p : L.Semiformula n) : p.shift.val = L.shift p.val := rfl
+@[simp] lemma val_substs (p : L.Semiformula n) (w : L.TSemitermVec n m) : (p.substs w).val = L.substs w.val p.val := rfl
 
-@[simp] lemma shift_verum : (⊤ : L.TSemiformula n).shift = ⊤ := by ext; simp [shift]
-@[simp] lemma shift_falsum : (⊥ : L.TSemiformula n).shift = ⊥ := by ext; simp [shift]
-@[simp] lemma shift_and (p q : L.TSemiformula n) : (p ⋏ q).shift = p.shift ⋏ q.shift := by ext; simp [shift]
-@[simp] lemma shift_or (p q : L.TSemiformula n) : (p ⋎ q).shift = p.shift ⋎ q.shift := by ext; simp [shift]
-@[simp] lemma shift_all (p : L.TSemiformula (n + 1)) : p.all.shift = p.shift.all := by ext; simp [shift]
-@[simp] lemma shift_ex (p : L.TSemiformula (n + 1)) : p.ex.shift = p.shift.ex := by ext; simp [shift]
+@[simp] lemma shift_verum : (⊤ : L.Semiformula n).shift = ⊤ := by ext; simp [shift]
+@[simp] lemma shift_falsum : (⊥ : L.Semiformula n).shift = ⊥ := by ext; simp [shift]
+@[simp] lemma shift_and (p q : L.Semiformula n) : (p ⋏ q).shift = p.shift ⋏ q.shift := by ext; simp [shift]
+@[simp] lemma shift_or (p q : L.Semiformula n) : (p ⋎ q).shift = p.shift ⋎ q.shift := by ext; simp [shift]
+@[simp] lemma shift_all (p : L.Semiformula (n + 1)) : p.all.shift = p.shift.all := by ext; simp [shift]
+@[simp] lemma shift_ex (p : L.Semiformula (n + 1)) : p.ex.shift = p.shift.ex := by ext; simp [shift]
 
-@[simp] lemma neg_inj {p q : L.TSemiformula n} :
+@[simp] lemma neg_inj {p q : L.Semiformula n} :
     ~p = ~q ↔ p = q :=
   ⟨by intro h; simpa using congr_arg (~·) h, by rintro rfl; rfl⟩
 
-@[simp] lemma imp_inj {p₁ p₂ q₁ q₂ : L.TSemiformula n} :
+@[simp] lemma imp_inj {p₁ p₂ q₁ q₂ : L.Semiformula n} :
     p₁ ⟶ p₂ = q₁ ⟶ q₂ ↔ p₁ = q₁ ∧ p₂ = q₂ := by simp [imp_def]
 
-@[simp] lemma shift_neg (p : L.TSemiformula n) : (~p).shift = ~(p.shift) := by
+@[simp] lemma shift_neg (p : L.Semiformula n) : (~p).shift = ~(p.shift) := by
   ext; simp [shift, val_neg, TSemitermVec.prop]
   rw [Arith.shift_neg p.prop]
-@[simp] lemma shift_imp (p q : L.TSemiformula n) : (p ⟶ q).shift = p.shift ⟶ q.shift := by
+@[simp] lemma shift_imp (p q : L.Semiformula n) : (p ⟶ q).shift = p.shift ⟶ q.shift := by
   simp [imp_def]
 
-@[simp] lemma substs_verum (w : L.TSemitermVec n m) : (⊤ : L.TSemiformula n).substs w = ⊤ := by ext; simp [substs]
-@[simp] lemma substs_falsum (w : L.TSemitermVec n m) : (⊥ : L.TSemiformula n).substs w = ⊥ := by ext; simp [substs]
-@[simp] lemma substs_and (w : L.TSemitermVec n m) (p q : L.TSemiformula n) :
+@[simp] lemma substs_verum (w : L.TSemitermVec n m) : (⊤ : L.Semiformula n).substs w = ⊤ := by ext; simp [substs]
+@[simp] lemma substs_falsum (w : L.TSemitermVec n m) : (⊥ : L.Semiformula n).substs w = ⊥ := by ext; simp [substs]
+@[simp] lemma substs_and (w : L.TSemitermVec n m) (p q : L.Semiformula n) :
     (p ⋏ q).substs w = p.substs w ⋏ q.substs w := by ext; simp [substs]
-@[simp] lemma substs_or (w : L.TSemitermVec n m) (p q : L.TSemiformula n) :
+@[simp] lemma substs_or (w : L.TSemitermVec n m) (p q : L.Semiformula n) :
     (p ⋎ q).substs w = p.substs w ⋎ q.substs w := by ext; simp [substs]
-@[simp] lemma substs_all (w : L.TSemitermVec n m) (p : L.TSemiformula (n + 1)) :
+@[simp] lemma substs_all (w : L.TSemitermVec n m) (p : L.Semiformula (n + 1)) :
     p.all.substs w = (p.substs w.q).all := by
   ext; simp [substs, Language.bvar, Language.qVec, Language.TSemitermVec.bShift, Language.TSemitermVec.q, w.prop.lh]
-@[simp] lemma substs_ex (w : L.TSemitermVec n m) (p : L.TSemiformula (n + 1)) :
+@[simp] lemma substs_ex (w : L.TSemitermVec n m) (p : L.Semiformula (n + 1)) :
     p.ex.substs w = (p.substs w.q).ex := by
   ext; simp [substs, Language.bvar, Language.qVec, Language.TSemitermVec.bShift, Language.TSemitermVec.q, w.prop.lh]
 
-@[simp] lemma substs_neg (w : L.TSemitermVec n m) (p : L.TSemiformula n) : (~p).substs w = ~(p.substs w) := by
+@[simp] lemma substs_neg (w : L.TSemitermVec n m) (p : L.Semiformula n) : (~p).substs w = ~(p.substs w) := by
   ext; simp [substs, val_neg, TSemitermVec.prop, Arith.substs_neg p.prop w.prop]
-@[simp] lemma substs_imp (w : L.TSemitermVec n m) (p q : L.TSemiformula n) : (p ⟶ q).substs w = p.substs w ⟶ q.substs w := by
+@[simp] lemma substs_imp (w : L.TSemitermVec n m) (p q : L.Semiformula n) : (p ⟶ q).substs w = p.substs w ⟶ q.substs w := by
   simp [imp_def]
-@[simp] lemma substs_imply (w : L.TSemitermVec n m) (p q : L.TSemiformula n) : (p ⟷ q).substs w = p.substs w ⟷ q.substs w := by
+@[simp] lemma substs_imply (w : L.TSemitermVec n m) (p q : L.Semiformula n) : (p ⟷ q).substs w = p.substs w ⟷ q.substs w := by
   simp [LogicalConnective.iff]
 
-end Language.TSemiformula
+end Language.Semiformula
 
-notation p:max "^/[" w "]" => Language.TSemiformula.substs p w
+notation p:max "^/[" w "]" => Language.Semiformula.substs p w
 
-structure Language.TSemiformulaVec (n : V) where
+structure Language.SemiformulaVec (n : V) where
   val : V
   prop : ∀ i < len val, L.IsSemiformula n val.[i]
 
-namespace Language.TSemiformulaVec
+namespace Language.SemiformulaVec
 
-def conj (ps : L.TSemiformulaVec n) : L.TSemiformula n := ⟨^⋀ ps.val, by simpa using ps.prop⟩
+def conj (ps : L.SemiformulaVec n) : L.Semiformula n := ⟨^⋀ ps.val, by simpa using ps.prop⟩
 
-def disj (ps : L.TSemiformulaVec n) : L.TSemiformula n := ⟨^⋁ ps.val, by simpa using ps.prop⟩
+def disj (ps : L.SemiformulaVec n) : L.Semiformula n := ⟨^⋁ ps.val, by simpa using ps.prop⟩
 
-def nth (ps : L.TSemiformulaVec n) (i : V) (hi : i < len ps.val) : L.TSemiformula n :=
+def nth (ps : L.SemiformulaVec n) (i : V) (hi : i < len ps.val) : L.Semiformula n :=
   ⟨ps.val.[i], ps.prop i hi⟩
 
-@[simp] lemma val_conj (ps : L.TSemiformulaVec n) : ps.conj.val = ^⋀ ps.val := rfl
+@[simp] lemma val_conj (ps : L.SemiformulaVec n) : ps.conj.val = ^⋀ ps.val := rfl
 
-@[simp] lemma val_disj (ps : L.TSemiformulaVec n) : ps.disj.val = ^⋁ ps.val := rfl
+@[simp] lemma val_disj (ps : L.SemiformulaVec n) : ps.disj.val = ^⋁ ps.val := rfl
 
-@[simp] lemma val_nth (ps : L.TSemiformulaVec n) (i : V) (hi : i < len ps.val) :
+@[simp] lemma val_nth (ps : L.SemiformulaVec n) (i : V) (hi : i < len ps.val) :
     (ps.nth i hi).val = ps.val.[i] := rfl
 
-end Language.TSemiformulaVec
+end Language.SemiformulaVec
 
 namespace Language.TSemifromula
 
-lemma subst_eq_self {n : V} (w : L.TSemitermVec n n) (p : L.TSemiformula n) (H : ∀ i, (hi : i < n) → w.nth i hi = L.bvar i hi) :
+lemma subst_eq_self {n : V} (w : L.TSemitermVec n n) (p : L.Semiformula n) (H : ∀ i, (hi : i < n) → w.nth i hi = L.bvar i hi) :
     p^/[w] = p := by
   ext; simp; rw [Arith.subst_eq_self p.prop w.prop]
   intro i hi
   simpa using congr_arg Language.Semiterm.val (H i hi)
 
-@[simp] lemma subst_eq_self₁ (p : L.TSemiformula (0 + 1)) :
+@[simp] lemma subst_eq_self₁ (p : L.Semiformula (0 + 1)) :
     p^/[(L.bvar 0 (by simp)).sing] = p := by
   apply subst_eq_self
   simp only [zero_add, lt_one_iff_eq_zero]
@@ -207,10 +207,10 @@ lemma subst_eq_self {n : V} (w : L.TSemitermVec n n) (p : L.TSemiformula n) (H :
 @[simp] lemma subst_nil_eq_self (w : L.TSemitermVec 0 0) :
     p^/[w] = p := subst_eq_self _ _ (by simp)
 
-lemma shift_substs {n m : V} (w : L.TSemitermVec n m) (p : L.TSemiformula n) :
+lemma shift_substs {n m : V} (w : L.TSemitermVec n m) (p : L.Semiformula n) :
     (p^/[w]).shift = p.shift^/[w.shift] := by ext; simp; rw [Arith.shift_substs p.prop w.prop]
 
-lemma substs_substs {n m l : V} (v : L.TSemitermVec m l) (w : L.TSemitermVec n m) (p : L.TSemiformula n) :
+lemma substs_substs {n m l : V} (v : L.TSemitermVec m l) (w : L.TSemitermVec n m) (p : L.Semiformula n) :
     (p^/[w])^/[v] = p^/[w.substs v] := by ext; simp; rw [Arith.substs_substs p.prop v.prop w.prop]
 
 end Language.TSemifromula
@@ -220,50 +220,50 @@ end typed_formula
 /-
 section typed_isfvfree
 
-namespace Language.TSemiformula
+namespace Language.Semiformula
 
-def FVFree (p : L.TSemiformula n) : Prop := L.IsFVFree n p.val
+def FVFree (p : L.Semiformula n) : Prop := L.IsFVFree n p.val
 
-lemma FVFree.iff {p : L.TSemiformula n} : p.FVFree ↔ p.shift = p := by
+lemma FVFree.iff {p : L.Semiformula n} : p.FVFree ↔ p.shift = p := by
   simp [FVFree, Language.IsFVFree, ext_iff]
 
-@[simp] lemma Fvfree.verum : (⊤ : L.TSemiformula n).FVFree := by simp [FVFree]
+@[simp] lemma Fvfree.verum : (⊤ : L.Semiformula n).FVFree := by simp [FVFree]
 
-@[simp] lemma Fvfree.falsum : (⊥ : L.TSemiformula n).FVFree := by simp [FVFree]
+@[simp] lemma Fvfree.falsum : (⊥ : L.Semiformula n).FVFree := by simp [FVFree]
 
-@[simp] lemma Fvfree.and {p q : L.TSemiformula n} :
+@[simp] lemma Fvfree.and {p q : L.Semiformula n} :
     (p ⋏ q).FVFree ↔ p.FVFree ∧ q.FVFree := by
   simp [FVFree.iff, FVFree.iff]
 
-@[simp] lemma Fvfree.or {p q : L.TSemiformula n} : (p ⋎ q).FVFree ↔ p.FVFree ∧ q.FVFree := by
+@[simp] lemma Fvfree.or {p q : L.Semiformula n} : (p ⋎ q).FVFree ↔ p.FVFree ∧ q.FVFree := by
   simp [FVFree.iff]
 
-@[simp] lemma Fvfree.neg {p : L.TSemiformula n} : (~p).FVFree ↔ p.FVFree := by
+@[simp] lemma Fvfree.neg {p : L.Semiformula n} : (~p).FVFree ↔ p.FVFree := by
   simp [FVFree.iff]
 
-@[simp] lemma Fvfree.all {p : L.TSemiformula (n + 1)} : p.all.FVFree ↔ p.FVFree := by
+@[simp] lemma Fvfree.all {p : L.Semiformula (n + 1)} : p.all.FVFree ↔ p.FVFree := by
   simp [FVFree.iff]
 
-@[simp] lemma Fvfree.ex {p : L.TSemiformula (n + 1)} : p.ex.FVFree ↔ p.FVFree := by
+@[simp] lemma Fvfree.ex {p : L.Semiformula (n + 1)} : p.ex.FVFree ↔ p.FVFree := by
   simp [FVFree.iff]
 
-@[simp] lemma Fvfree.imp {p q : L.TSemiformula n} : (p ⟶ q).FVFree ↔ p.FVFree ∧ q.FVFree := by
+@[simp] lemma Fvfree.imp {p q : L.Semiformula n} : (p ⟶ q).FVFree ↔ p.FVFree ∧ q.FVFree := by
   simp [FVFree.iff]
 
-end Language.TSemiformula
+end Language.Semiformula
 
 end typed_isfvfree
 -/
 
 open Formalized
 
-def Language.Semiterm.equals {n : V} (t u : ⌜ℒₒᵣ⌝.Semiterm n) : ⌜ℒₒᵣ⌝.TSemiformula n := ⟨t.val ^= u.val, by simp [qqEQ]⟩
+def Language.Semiterm.equals {n : V} (t u : ⌜ℒₒᵣ⌝.Semiterm n) : ⌜ℒₒᵣ⌝.Semiformula n := ⟨t.val ^= u.val, by simp [qqEQ]⟩
 
-def Language.Semiterm.notEquals {n : V} (t u : ⌜ℒₒᵣ⌝.Semiterm n) : ⌜ℒₒᵣ⌝.TSemiformula n := ⟨t.val ^≠ u.val, by simp [qqNEQ]⟩
+def Language.Semiterm.notEquals {n : V} (t u : ⌜ℒₒᵣ⌝.Semiterm n) : ⌜ℒₒᵣ⌝.Semiformula n := ⟨t.val ^≠ u.val, by simp [qqNEQ]⟩
 
-def Language.Semiterm.lessThan {n : V} (t u : ⌜ℒₒᵣ⌝.Semiterm n) : ⌜ℒₒᵣ⌝.TSemiformula n := ⟨t.val ^< u.val, by simp [qqLT]⟩
+def Language.Semiterm.lessThan {n : V} (t u : ⌜ℒₒᵣ⌝.Semiterm n) : ⌜ℒₒᵣ⌝.Semiformula n := ⟨t.val ^< u.val, by simp [qqLT]⟩
 
-def Language.Semiterm.notLessThan {n : V} (t u : ⌜ℒₒᵣ⌝.Semiterm n) : ⌜ℒₒᵣ⌝.TSemiformula n := ⟨t.val ^≮ u.val, by simp [qqNLT]⟩
+def Language.Semiterm.notLessThan {n : V} (t u : ⌜ℒₒᵣ⌝.Semiterm n) : ⌜ℒₒᵣ⌝.Semiformula n := ⟨t.val ^≮ u.val, by simp [qqNLT]⟩
 
 scoped infix:75 " =' " => Language.Semiterm.equals
 
@@ -273,10 +273,10 @@ scoped infix:75 " <' " => Language.Semiterm.lessThan
 
 scoped infix:75 " ≮' " => Language.Semiterm.notLessThan
 
-def Language.TSemiformula.ball {n : V} (t : ⌜ℒₒᵣ⌝.Semiterm n) (p : ⌜ℒₒᵣ⌝.TSemiformula (n + 1)) : ⌜ℒₒᵣ⌝.TSemiformula n :=
+def Language.Semiformula.ball {n : V} (t : ⌜ℒₒᵣ⌝.Semiterm n) (p : ⌜ℒₒᵣ⌝.Semiformula (n + 1)) : ⌜ℒₒᵣ⌝.Semiformula n :=
   (⌜ℒₒᵣ⌝.bvar 0 ≮' t.bShift ⋎ p).all
 
-def Language.TSemiformula.bex {n : V} (t : ⌜ℒₒᵣ⌝.Semiterm n) (p : ⌜ℒₒᵣ⌝.TSemiformula (n + 1)) : ⌜ℒₒᵣ⌝.TSemiformula n :=
+def Language.Semiformula.bex {n : V} (t : ⌜ℒₒᵣ⌝.Semiterm n) (p : ⌜ℒₒᵣ⌝.Semiformula (n + 1)) : ⌜ℒₒᵣ⌝.Semiformula n :=
   (⌜ℒₒᵣ⌝.bvar 0 <' t.bShift ⋏ p).ex
 
 namespace Formalized
@@ -290,19 +290,19 @@ variable {n m : V}
 
 @[simp] lemma equals_iff {t₁ t₂ u₁ u₂ : ⌜ℒₒᵣ⌝.Semiterm n} :
     (t₁ =' u₁) = (t₂ =' u₂) ↔ t₁ = t₂ ∧ u₁ = u₂ := by
-  simp [Language.TSemiformula.ext_iff, Language.Semiterm.ext_iff, qqEQ]
+  simp [Language.Semiformula.ext_iff, Language.Semiterm.ext_iff, qqEQ]
 
 @[simp] lemma notequals_iff {t₁ t₂ u₁ u₂ : ⌜ℒₒᵣ⌝.Semiterm n} :
     (t₁ ≠' u₁) = (t₂ ≠' u₂) ↔ t₁ = t₂ ∧ u₁ = u₂ := by
-  simp [Language.TSemiformula.ext_iff, Language.Semiterm.ext_iff, qqNEQ]
+  simp [Language.Semiformula.ext_iff, Language.Semiterm.ext_iff, qqNEQ]
 
 @[simp] lemma lessThan_iff {t₁ t₂ u₁ u₂ : ⌜ℒₒᵣ⌝.Semiterm n} :
     (t₁ <' u₁) = (t₂ <' u₂) ↔ t₁ = t₂ ∧ u₁ = u₂ := by
-  simp [Language.TSemiformula.ext_iff, Language.Semiterm.ext_iff, qqLT]
+  simp [Language.Semiformula.ext_iff, Language.Semiterm.ext_iff, qqLT]
 
 @[simp] lemma notLessThan_iff {t₁ t₂ u₁ u₂ : ⌜ℒₒᵣ⌝.Semiterm n} :
     (t₁ ≮' u₁) = (t₂ ≮' u₂) ↔ t₁ = t₂ ∧ u₁ = u₂ := by
-  simp [Language.TSemiformula.ext_iff, Language.Semiterm.ext_iff, qqNLT]
+  simp [Language.Semiformula.ext_iff, Language.Semiterm.ext_iff, qqNLT]
 
 @[simp] lemma neg_equals (t₁ t₂ : ⌜ℒₒᵣ⌝.Semiterm n) :
     ~(t₁ =' t₂) = (t₁ ≠' t₂) := by
@@ -322,123 +322,123 @@ variable {n m : V}
 
 @[simp] lemma shift_equals (t₁ t₂ : ⌜ℒₒᵣ⌝.Semiterm n) :
     (t₁ =' t₂).shift = (t₁.shift =' t₂.shift) := by
-  ext; simp [Language.Semiterm.equals, Language.Semiterm.shift, Language.TSemiformula.shift, qqEQ]
+  ext; simp [Language.Semiterm.equals, Language.Semiterm.shift, Language.Semiformula.shift, qqEQ]
 
 @[simp] lemma shift_notEquals (t₁ t₂ : ⌜ℒₒᵣ⌝.Semiterm n) :
     (t₁ ≠' t₂).shift = (t₁.shift ≠' t₂.shift) := by
-  ext; simp [Language.Semiterm.notEquals, Language.Semiterm.shift, Language.TSemiformula.shift, qqNEQ]
+  ext; simp [Language.Semiterm.notEquals, Language.Semiterm.shift, Language.Semiformula.shift, qqNEQ]
 
 @[simp] lemma shift_lessThan (t₁ t₂ : ⌜ℒₒᵣ⌝.Semiterm n) :
     (t₁ <' t₂).shift = (t₁.shift <' t₂.shift) := by
-  ext; simp [Language.Semiterm.lessThan, Language.Semiterm.shift, Language.TSemiformula.shift, qqLT]
+  ext; simp [Language.Semiterm.lessThan, Language.Semiterm.shift, Language.Semiformula.shift, qqLT]
 
 @[simp] lemma shift_notLessThan (t₁ t₂ : ⌜ℒₒᵣ⌝.Semiterm n) :
     (t₁ ≮' t₂).shift = (t₁.shift ≮' t₂.shift) := by
-  ext; simp [Language.Semiterm.notLessThan, Language.Semiterm.shift, Language.TSemiformula.shift, qqNLT]
+  ext; simp [Language.Semiterm.notLessThan, Language.Semiterm.shift, Language.Semiformula.shift, qqNLT]
 
 @[simp] lemma substs_equals (w : ⌜ℒₒᵣ⌝.TSemitermVec n m) (t₁ t₂ : ⌜ℒₒᵣ⌝.Semiterm n) :
     (t₁ =' t₂).substs w = (t₁.substs w =' t₂.substs w) := by
-  ext; simp [Language.Semiterm.equals, Language.Semiterm.substs, Language.TSemiformula.substs, qqEQ]
+  ext; simp [Language.Semiterm.equals, Language.Semiterm.substs, Language.Semiformula.substs, qqEQ]
 
 @[simp] lemma substs_notEquals (w : ⌜ℒₒᵣ⌝.TSemitermVec n m) (t₁ t₂ : ⌜ℒₒᵣ⌝.Semiterm n) :
     (t₁ ≠' t₂).substs w = (t₁.substs w ≠' t₂.substs w) := by
-  ext; simp [Language.Semiterm.notEquals, Language.Semiterm.substs, Language.TSemiformula.substs, qqNEQ]
+  ext; simp [Language.Semiterm.notEquals, Language.Semiterm.substs, Language.Semiformula.substs, qqNEQ]
 
 @[simp] lemma substs_lessThan (w : ⌜ℒₒᵣ⌝.TSemitermVec n m) (t₁ t₂ : ⌜ℒₒᵣ⌝.Semiterm n) :
     (t₁ <' t₂).substs w = (t₁.substs w <' t₂.substs w) := by
-  ext; simp [Language.Semiterm.lessThan, Language.Semiterm.substs, Language.TSemiformula.substs, qqLT]
+  ext; simp [Language.Semiterm.lessThan, Language.Semiterm.substs, Language.Semiformula.substs, qqLT]
 
 @[simp] lemma substs_notLessThan (w : ⌜ℒₒᵣ⌝.TSemitermVec n m) (t₁ t₂ : ⌜ℒₒᵣ⌝.Semiterm n) :
     (t₁ ≮' t₂).substs w = (t₁.substs w ≮' t₂.substs w) := by
-  ext; simp [Language.Semiterm.notLessThan, Language.Semiterm.substs, Language.TSemiformula.substs, qqNLT]
+  ext; simp [Language.Semiterm.notLessThan, Language.Semiterm.substs, Language.Semiformula.substs, qqNLT]
 
-@[simp] lemma val_ball {n : V} (t : ⌜ℒₒᵣ⌝.Semiterm n) (p : ⌜ℒₒᵣ⌝.TSemiformula (n + 1)) :
+@[simp] lemma val_ball {n : V} (t : ⌜ℒₒᵣ⌝.Semiterm n) (p : ⌜ℒₒᵣ⌝.Semiformula (n + 1)) :
     (p.ball t).val = ^∀ (^#0 ^≮ ⌜ℒₒᵣ⌝.termBShift t.val) ^⋎ p.val := by
-  simp [Language.TSemiformula.ball]
+  simp [Language.Semiformula.ball]
 
-@[simp] lemma val_bex {n : V} (t : ⌜ℒₒᵣ⌝.Semiterm n) (p : ⌜ℒₒᵣ⌝.TSemiformula (n + 1)) :
+@[simp] lemma val_bex {n : V} (t : ⌜ℒₒᵣ⌝.Semiterm n) (p : ⌜ℒₒᵣ⌝.Semiformula (n + 1)) :
     (p.bex t).val = ^∃ (^#0 ^< ⌜ℒₒᵣ⌝.termBShift t.val) ^⋏ p.val := by
-  simp [Language.TSemiformula.bex]
+  simp [Language.Semiformula.bex]
 
-lemma neg_ball (t : ⌜ℒₒᵣ⌝.Semiterm n) (p : ⌜ℒₒᵣ⌝.TSemiformula (n + 1)) :
+lemma neg_ball (t : ⌜ℒₒᵣ⌝.Semiterm n) (p : ⌜ℒₒᵣ⌝.Semiformula (n + 1)) :
     ~(p.ball t) = (~p).bex t := by
   ext; simp; rw [neg_all, neg_or] <;> simp [qqNLT, qqLT, t.prop.termBShift.isUTerm]
 
-lemma neg_bex (t : ⌜ℒₒᵣ⌝.Semiterm n) (p : ⌜ℒₒᵣ⌝.TSemiformula (n + 1)) :
+lemma neg_bex (t : ⌜ℒₒᵣ⌝.Semiterm n) (p : ⌜ℒₒᵣ⌝.Semiformula (n + 1)) :
     ~(p.bex t) = (~p).ball t := by
   ext; simp; rw [neg_ex, neg_and] <;> simp [qqNLT, qqLT, t.prop.termBShift.isUTerm]
 
-@[simp] lemma shifts_ball (t : ⌜ℒₒᵣ⌝.Semiterm n) (p : ⌜ℒₒᵣ⌝.TSemiformula (n + 1)) :
+@[simp] lemma shifts_ball (t : ⌜ℒₒᵣ⌝.Semiterm n) (p : ⌜ℒₒᵣ⌝.Semiformula (n + 1)) :
     (p.ball t).shift = p.shift.ball t.shift := by
-  simp [Language.TSemiformula.ball, Language.Semiterm.bShift_shift_comm]
+  simp [Language.Semiformula.ball, Language.Semiterm.bShift_shift_comm]
 
-@[simp] lemma shifts_bex (t : ⌜ℒₒᵣ⌝.Semiterm n) (p : ⌜ℒₒᵣ⌝.TSemiformula (n + 1)) :
+@[simp] lemma shifts_bex (t : ⌜ℒₒᵣ⌝.Semiterm n) (p : ⌜ℒₒᵣ⌝.Semiformula (n + 1)) :
     (p.bex t).shift = p.shift.bex t.shift := by
-  simp [Language.TSemiformula.bex, Language.Semiterm.bShift_shift_comm]
+  simp [Language.Semiformula.bex, Language.Semiterm.bShift_shift_comm]
 
-@[simp] lemma substs_ball (w : ⌜ℒₒᵣ⌝.TSemitermVec n m) (t : ⌜ℒₒᵣ⌝.Semiterm n) (p : ⌜ℒₒᵣ⌝.TSemiformula (n + 1)) :
+@[simp] lemma substs_ball (w : ⌜ℒₒᵣ⌝.TSemitermVec n m) (t : ⌜ℒₒᵣ⌝.Semiterm n) (p : ⌜ℒₒᵣ⌝.Semiformula (n + 1)) :
     (p.ball t)^/[w] = (p^/[w.q]).ball (t^ᵗ/[w]) := by
-  simp [Language.TSemiformula.ball]
+  simp [Language.Semiformula.ball]
 
-@[simp] lemma substs_bex (w : ⌜ℒₒᵣ⌝.TSemitermVec n m) (t : ⌜ℒₒᵣ⌝.Semiterm n) (p : ⌜ℒₒᵣ⌝.TSemiformula (n + 1)) :
+@[simp] lemma substs_bex (w : ⌜ℒₒᵣ⌝.TSemitermVec n m) (t : ⌜ℒₒᵣ⌝.Semiterm n) (p : ⌜ℒₒᵣ⌝.Semiformula (n + 1)) :
     (p.bex t)^/[w] = (p^/[w.q]).bex (t^ᵗ/[w]) := by
-  simp [Language.TSemiformula.bex]
+  simp [Language.Semiformula.bex]
 
-def tSubstItr {n m : V} (w : ⌜ℒₒᵣ⌝.TSemitermVec n m) (p : ⌜ℒₒᵣ⌝.TSemiformula (n + 1)) (k : V) :
-    ⌜ℒₒᵣ⌝.TSemiformulaVec m := ⟨substItr w.val p.val k, by
+def tSubstItr {n m : V} (w : ⌜ℒₒᵣ⌝.TSemitermVec n m) (p : ⌜ℒₒᵣ⌝.Semiformula (n + 1)) (k : V) :
+    ⌜ℒₒᵣ⌝.SemiformulaVec m := ⟨substItr w.val p.val k, by
   intro i hi
   have : i < k := by simpa using hi
   simp only [gt_iff_lt, this, substItr_nth]
   exact p.prop.substs (w.prop.cons (by simp))⟩
 
-@[simp] lemma val_tSubstItr {n m : V} (w : ⌜ℒₒᵣ⌝.TSemitermVec n m) (p : ⌜ℒₒᵣ⌝.TSemiformula (n + 1)) (k : V) :
+@[simp] lemma val_tSubstItr {n m : V} (w : ⌜ℒₒᵣ⌝.TSemitermVec n m) (p : ⌜ℒₒᵣ⌝.Semiformula (n + 1)) (k : V) :
     (tSubstItr w p k).val = substItr w.val p.val k := by simp [tSubstItr]
 
-@[simp] lemma len_tSubstItr {n m : V} (w : ⌜ℒₒᵣ⌝.TSemitermVec n m) (p : ⌜ℒₒᵣ⌝.TSemiformula (n + 1)) (k : V) :
+@[simp] lemma len_tSubstItr {n m : V} (w : ⌜ℒₒᵣ⌝.TSemitermVec n m) (p : ⌜ℒₒᵣ⌝.Semiformula (n + 1)) (k : V) :
     len (tSubstItr w p k).val = k := by simp
 
-lemma nth_tSubstItr {n m : V} (w : ⌜ℒₒᵣ⌝.TSemitermVec n m) (p : ⌜ℒₒᵣ⌝.TSemiformula (n + 1)) (k : V) {i} (hi : i < k) :
-    (tSubstItr w p k).nth i (by simp [hi]) = p.substs (↑(k - (i + 1)) ∷ᵗ w) := by ext; simp [tSubstItr, Language.TSemiformula.substs, hi]
+lemma nth_tSubstItr {n m : V} (w : ⌜ℒₒᵣ⌝.TSemitermVec n m) (p : ⌜ℒₒᵣ⌝.Semiformula (n + 1)) (k : V) {i} (hi : i < k) :
+    (tSubstItr w p k).nth i (by simp [hi]) = p.substs (↑(k - (i + 1)) ∷ᵗ w) := by ext; simp [tSubstItr, Language.Semiformula.substs, hi]
 
-lemma nth_tSubstItr' {n m : V} (w : ⌜ℒₒᵣ⌝.TSemitermVec n m) (p : ⌜ℒₒᵣ⌝.TSemiformula (n + 1)) (k : V) {i} (hi : i < k) :
+lemma nth_tSubstItr' {n m : V} (w : ⌜ℒₒᵣ⌝.TSemitermVec n m) (p : ⌜ℒₒᵣ⌝.Semiformula (n + 1)) (k : V) {i} (hi : i < k) :
     (tSubstItr w p k).nth (k - (i + 1)) (by simpa using sub_succ_lt_self hi) = p.substs (↑i ∷ᵗ w) := by
-  ext; simp [tSubstItr, Language.TSemiformula.substs, hi, sub_succ_lt_self hi, sub_succ_lt_selfs hi]
+  ext; simp [tSubstItr, Language.Semiformula.substs, hi, sub_succ_lt_self hi, sub_succ_lt_selfs hi]
 
-@[simp] lemma neg_conj_tSubstItr {n m : V} (w : ⌜ℒₒᵣ⌝.TSemitermVec n m) (p : ⌜ℒₒᵣ⌝.TSemiformula (n + 1)) (k : V) :
+@[simp] lemma neg_conj_tSubstItr {n m : V} (w : ⌜ℒₒᵣ⌝.TSemitermVec n m) (p : ⌜ℒₒᵣ⌝.Semiformula (n + 1)) (k : V) :
     ~(tSubstItr w p k).conj = (tSubstItr w (~p) k).disj := by
   ext; simp [neg_conj_substItr p.prop w.prop]
 
-@[simp] lemma neg_disj_tSubstItr {n m : V} (w : ⌜ℒₒᵣ⌝.TSemitermVec n m) (p : ⌜ℒₒᵣ⌝.TSemiformula (n + 1)) (k : V) :
+@[simp] lemma neg_disj_tSubstItr {n m : V} (w : ⌜ℒₒᵣ⌝.TSemitermVec n m) (p : ⌜ℒₒᵣ⌝.Semiformula (n + 1)) (k : V) :
     ~(tSubstItr w p k).disj = (tSubstItr w (~p) k).conj := by
   ext; simp [neg_disj_substItr p.prop w.prop]
 
-@[simp] lemma substs_conj_tSubstItr {n m l : V} (v : ⌜ℒₒᵣ⌝.TSemitermVec m l) (w : ⌜ℒₒᵣ⌝.TSemitermVec n m) (p : ⌜ℒₒᵣ⌝.TSemiformula (n + 1)) (k : V) :
+@[simp] lemma substs_conj_tSubstItr {n m l : V} (v : ⌜ℒₒᵣ⌝.TSemitermVec m l) (w : ⌜ℒₒᵣ⌝.TSemitermVec n m) (p : ⌜ℒₒᵣ⌝.Semiformula (n + 1)) (k : V) :
     (tSubstItr w p k).conj.substs v = (tSubstItr (w.substs v) p k).conj := by
-  ext; simp [Language.TSemiformula.substs, Language.TSemitermVec.substs]
+  ext; simp [Language.Semiformula.substs, Language.TSemitermVec.substs]
   rw [substs_conj_substItr p.prop w.prop v.prop]
 
-@[simp] lemma substs_disj_tSubstItr {n m l : V} (v : ⌜ℒₒᵣ⌝.TSemitermVec m l) (w : ⌜ℒₒᵣ⌝.TSemitermVec n m) (p : ⌜ℒₒᵣ⌝.TSemiformula (n + 1)) (k : V) :
+@[simp] lemma substs_disj_tSubstItr {n m l : V} (v : ⌜ℒₒᵣ⌝.TSemitermVec m l) (w : ⌜ℒₒᵣ⌝.TSemitermVec n m) (p : ⌜ℒₒᵣ⌝.Semiformula (n + 1)) (k : V) :
     (tSubstItr w p k).disj.substs v = (tSubstItr (w.substs v) p k).disj := by
-  ext; simp [Language.TSemiformula.substs, Language.TSemitermVec.substs]
+  ext; simp [Language.Semiformula.substs, Language.TSemitermVec.substs]
   rw [substs_disj_substItr p.prop w.prop v.prop]
 
 /-
 @[simp] lemma equals_fvfree {t u : ⌜ℒₒᵣ⌝.Semiterm n} : (t =' u).FVFree ↔ t.FVFree ∧ u.FVFree := by
-  simp [Language.TSemiformula.FVFree.iff, Language.Semiterm.FVFree.iff]
+  simp [Language.Semiformula.FVFree.iff, Language.Semiterm.FVFree.iff]
 
 @[simp] lemma notEquals_fvfree {t u : ⌜ℒₒᵣ⌝.Semiterm n} : (t ≠' u).FVFree ↔ t.FVFree ∧ u.FVFree := by
-  simp [Language.TSemiformula.FVFree.iff, Language.Semiterm.FVFree.iff]
+  simp [Language.Semiformula.FVFree.iff, Language.Semiterm.FVFree.iff]
 
 @[simp] lemma lessThan_fvfree {t u : ⌜ℒₒᵣ⌝.Semiterm n} : (t <' u).FVFree ↔ t.FVFree ∧ u.FVFree := by
-  simp [Language.TSemiformula.FVFree.iff, Language.Semiterm.FVFree.iff]
+  simp [Language.Semiformula.FVFree.iff, Language.Semiterm.FVFree.iff]
 
 @[simp] lemma notLessThan_fvfree {t u : ⌜ℒₒᵣ⌝.Semiterm n} : (t ≮' u).FVFree ↔ t.FVFree ∧ u.FVFree := by
-  simp [Language.TSemiformula.FVFree.iff, Language.Semiterm.FVFree.iff]
+  simp [Language.Semiformula.FVFree.iff, Language.Semiterm.FVFree.iff]
 -/
 
 end Formalized
 
-lemma Language.TSemiformula.ball_eq_imp {n : V} (t : ⌜ℒₒᵣ⌝.Semiterm n) (p : ⌜ℒₒᵣ⌝.TSemiformula (n + 1)) :
-    p.ball t = (⌜ℒₒᵣ⌝.bvar 0 <' t.bShift ⟶ p).all := by simp [Language.TSemiformula.ball, imp_def]
+lemma Language.Semiformula.ball_eq_imp {n : V} (t : ⌜ℒₒᵣ⌝.Semiterm n) (p : ⌜ℒₒᵣ⌝.Semiformula (n + 1)) :
+    p.ball t = (⌜ℒₒᵣ⌝.bvar 0 <' t.bShift ⟶ p).all := by simp [Language.Semiformula.ball, imp_def]
 
 end LO.Arith
